erasure/theories/Extraction.v
@@ -32,11 +32,13 @@ Extraction Inline Equations.Init.hidebody.
 Extraction Inline Equations.Prop.DepElim.solution_left.
 
 Extract Inductive Equations.Init.sigma => "( * )" ["(,)"].
+Extract Constant Equations.Init.pr1 => "fst".
+Extract Constant Equations.Init.pr2 => "snd".
+Extraction Inline Equations.Init.pr1 Equations.Init.pr2.
 
 Extract Constant PCUICTyping.fix_guard => "(fun x -> true)".
 Extract Constant PCUICTyping.cofix_guard => "(fun x -> true)".
 Extract Constant PCUICTyping.ind_guard => "(fun x -> true)".
-Extract Constant PCUICSafeChecker.check_one_ind_body => "(fun _ _ _ _ _ _ _ -> ret envcheck_monad __)".
 (* Extract Constant erase_mfix_obligation_1 => "(fun _ _ _ _ => ret typing_monad __)". *)
 
 Cd "src".
